proof: add context merging function + lemmas for let-bang

cogent/isa/ContextReconstruct.thy
@@ -2,16 +2,22 @@ theory ContextReconstruct
   imports Cogent
 begin
 
-fun merge_ctx :: "kind env \<Rightarrow> ctx \<Rightarrow> ctx \<Rightarrow> ctx" where
-  "merge_ctx K [] [] = []"
-| "merge_ctx K (Some x # \<Gamma>1) (Some y # \<Gamma>2) = (if (x = y) \<and> (\<exists>k. K \<turnstile> x :\<kappa> k \<and> S \<in> k)
-                                              then Some x # merge_ctx K \<Gamma>1 \<Gamma>2
-                                              else undefined)"
-| "merge_ctx K (Some x # \<Gamma>1) (None # \<Gamma>2) = Some x # merge_ctx K \<Gamma>1 \<Gamma>2"
-| "merge_ctx K (None # \<Gamma>1) (Some y # \<Gamma>2) = Some y # merge_ctx K \<Gamma>1 \<Gamma>2"
-| "merge_ctx K (None # \<Gamma>1) (None # \<Gamma>2) = None # merge_ctx K \<Gamma>1 \<Gamma>2"
+section {* Functions for merging split contexts *}
+text {* These will give back undefined-s in strange places if the contexts can't actually be merged. *}
 
-lemma merge_ctx_correct:
+fun merge_ctx_comp :: "kind env \<Rightarrow> type option \<Rightarrow> type option \<Rightarrow> type option" where
+  "merge_ctx_comp K (Some x) (Some y) = (if (x = y) \<and> (\<exists>k. K \<turnstile> x :\<kappa> k \<and> S \<in> k)
+                                              then Some x
+                                              else undefined)"
+| "merge_ctx_comp K (Some x) (None) = Some x"
+| "merge_ctx_comp K (None) (Some y) = Some y"
+| "merge_ctx_comp K (None) (None) = None"
+
+fun merge_ctx :: "kind env \<Rightarrow> ctx \<Rightarrow> ctx \<Rightarrow> ctx" where
+  "merge_ctx _ [] [] = []"
+| "merge_ctx K (optx # \<Gamma>1) (opty # \<Gamma>2) = merge_ctx_comp K optx opty # merge_ctx K \<Gamma>1 \<Gamma>2"
+
+lemma merge_ctx_correct_on_splits:
   assumes "K \<turnstile> \<Gamma> \<leadsto> \<Gamma>1 | \<Gamma>2"
   shows "\<Gamma> = merge_ctx K \<Gamma>1 \<Gamma>2"
   using assms
@@ -33,9 +39,31 @@ next
     using Cons.hyps split_comp.simps by auto
 qed
 
-fun merge_ctx_bang :: "nat set \<Rightarrow> kind env \<Rightarrow> ctx \<Rightarrow> ctx \<Rightarrow> ctx" where
-  "merge_ctx_bang _ _ _ = undefined"
+fun merge_ctx_bang_comp :: "kind env \<Rightarrow> bool \<Rightarrow> type option \<Rightarrow> type option \<Rightarrow> type option" where
+  "merge_ctx_bang_comp K False optx opty = merge_ctx_comp K optx opty"
+| "merge_ctx_bang_comp K True (Some x) (Some y) = (if x = bang y then Some y else undefined)"
 
+fun merge_ctx_bang :: "kind env \<Rightarrow> nat set \<Rightarrow> ctx \<Rightarrow> ctx \<Rightarrow> ctx" where
+  "merge_ctx_bang K is [] [] = []"
+| "merge_ctx_bang K is (optx # \<Gamma>1) (opty # \<Gamma>2) = (let is' = pred ` Set.remove (0 :: index) is
+                                                      in merge_ctx_bang_comp K (0 \<in> is) optx opty
+                                                        # merge_ctx_bang K is' \<Gamma>1 \<Gamma>2)"
+
+
+lemma merge_ctx_bang_correct_on_split_bangs:
+  assumes "split_bang K is \<Gamma> \<Gamma>1 \<Gamma>2"
+  shows "\<Gamma> = merge_ctx_bang K is \<Gamma>1 \<Gamma>2"
+  using assms
+proof (induct rule: split_bang.inducts)
+  case (split_bang_cons "is" K x a b \<Gamma> \<Gamma>1 \<Gamma>2)
+  moreover have
+    "x = merge_ctx_comp K a b"
+    "pred ` Set.remove 0 is = pred ` is"
+    using split_bang_cons.hyps split_comp.simps 
+    by (fastforce simp add: remove_def)+
+  ultimately show ?case 
+    by simp
+qed simp+
 
 inductive typing_minimal :: "('f \<Rightarrow> poly_type) \<Rightarrow> kind env \<Rightarrow> ctx \<Rightarrow> 'f expr \<Rightarrow> type \<Rightarrow> ctx \<Rightarrow> bool"
           ("_, _, _ \<turnstile> _ :m _ \<stileturn> _" [30,0,0,0,0,20] 60)
@@ -43,125 +71,337 @@ inductive typing_minimal :: "('f \<Rightarrow> poly_type) \<Rightarrow> kind env
           ("_, _, _ \<turnstile>* _ :m _ \<stileturn> _" [30,0,0,0,0,20] 60) where
 
   typing_min_var    : "\<lbrakk> i < length \<Gamma>
-                   \<rbrakk> \<Longrightarrow> \<Xi>, K, \<Gamma> \<turnstile> Var i :m t \<stileturn> singleton (length \<Gamma>) i t"
+                       ; K \<turnstile> \<Gamma> \<leadsto>w singleton (length \<Gamma>) i t (* correctness *)
+                       \<rbrakk> \<Longrightarrow> \<Xi>, K, \<Gamma> \<turnstile> Var i :m t \<stileturn> singleton (length \<Gamma>) i t"
 
 | typing_min_afun   : "\<lbrakk> \<Xi> f = (K', t, u)
-                   ; list_all2 (kinding K) ts K'
-                   ; K' \<turnstile> TFun t u wellformed
-                   \<rbrakk> \<Longrightarrow> \<Xi>, K, \<Gamma> \<turnstile> AFun f ts :m instantiate ts (TFun t u) \<stileturn> empty (length \<Gamma>)"
+                       ; list_all2 (kinding K) ts K'
+                       ; K' \<turnstile> TFun t u wellformed
+                       ; K \<turnstile> \<Gamma> \<leadsto>w empty (length \<Gamma>) (* correctness *)
+                       \<rbrakk> \<Longrightarrow> \<Xi>, K, \<Gamma> \<turnstile> AFun f ts :m instantiate ts (TFun t u) \<stileturn> empty (length \<Gamma>)"
 
 | typing_min_fun    : "\<lbrakk> \<Xi>, K', [Some t] \<turnstile> f :m u \<stileturn> \<Gamma>1'
-                   ; K' \<turnstile> t wellformed
-                   ; list_all2 (kinding K) ts K'
-                   \<rbrakk> \<Longrightarrow> \<Xi>, K, \<Gamma> \<turnstile> Fun f ts :m instantiate ts (TFun t u) \<stileturn> empty (length \<Gamma>)"
+                       ; K' \<turnstile> t wellformed
+                       ; list_all2 (kinding K) ts K'
+                       ; K \<turnstile> \<Gamma> \<leadsto>w empty (length \<Gamma>) (* correctness *)
+                       \<rbrakk> \<Longrightarrow> \<Xi>, K, \<Gamma> \<turnstile> Fun f ts :m instantiate ts (TFun t u) \<stileturn> empty (length \<Gamma>)"
 
 | typing_min_app    : "\<lbrakk> K \<turnstile> \<Gamma> \<leadsto> \<Gamma>1 | \<Gamma>2
-                   ; \<Xi>, K, \<Gamma>1 \<turnstile> a :m TFun x y \<stileturn> \<Gamma>1'
-                   ; \<Xi>, K, \<Gamma>2 \<turnstile> b :m x \<stileturn> \<Gamma>2'
-                   \<rbrakk> \<Longrightarrow> \<Xi>, K, \<Gamma> \<turnstile> App a b :m y \<stileturn> merge_ctx K \<Gamma>1 \<Gamma>2"
+                       ; \<Xi>, K, \<Gamma>1 \<turnstile> a :m TFun x y \<stileturn> \<Gamma>1'
+                       ; \<Xi>, K, \<Gamma>2 \<turnstile> b :m x \<stileturn> \<Gamma>2'
+                       \<rbrakk> \<Longrightarrow> \<Xi>, K, \<Gamma> \<turnstile> App a b :m y \<stileturn> merge_ctx K \<Gamma>1 \<Gamma>2"
 
 | typing_min_con    : "\<lbrakk> \<Xi>, K, \<Gamma> \<turnstile> x :m t \<stileturn> \<Gamma>'
-                   ; (tag, t, False) \<in> set ts
-                   ; K \<turnstile>* (map (fst \<circ> snd) ts) wellformed
-                   ; distinct (map fst ts)
-                   \<rbrakk> \<Longrightarrow> \<Xi>, K, \<Gamma> \<turnstile> Con ts tag x :m TSum ts \<stileturn> \<Gamma>'"
+                       ; (tag, t, False) \<in> set ts
+                       ; K \<turnstile>* (map (fst \<circ> snd) ts) wellformed
+                       ; distinct (map fst ts)
+                       \<rbrakk> \<Longrightarrow> \<Xi>, K, \<Gamma> \<turnstile> Con ts tag x :m TSum ts \<stileturn> \<Gamma>'"
 
 | typing_min_cast   : "\<lbrakk> \<Xi>, K, \<Gamma> \<turnstile> e :m TPrim (Num \<tau>) \<stileturn> \<Gamma>'
-                   ; upcast_valid \<tau> \<tau>'
-                   \<rbrakk> \<Longrightarrow> \<Xi>, K, \<Gamma> \<turnstile> Cast \<tau>' e :m TPrim (Num \<tau>') \<stileturn> \<Gamma>'"
+                       ; upcast_valid \<tau> \<tau>'
+                       \<rbrakk> \<Longrightarrow> \<Xi>, K, \<Gamma> \<turnstile> Cast \<tau>' e :m TPrim (Num \<tau>') \<stileturn> \<Gamma>'"
 
 | typing_min_tuple  : "\<lbrakk> K \<turnstile> \<Gamma> \<leadsto> \<Gamma>1 | \<Gamma>2
-                   ; \<Xi>, K, \<Gamma>1 \<turnstile> x :m t \<stileturn> \<Gamma>1'
-                   ; \<Xi>, K, \<Gamma>2 \<turnstile> y :m u \<stileturn> \<Gamma>2'
-                   \<rbrakk> \<Longrightarrow> \<Xi>, K, \<Gamma> \<turnstile> Tuple x y :m TProduct t u \<stileturn> merge_ctx K \<Gamma>1' \<Gamma>2'"
+                       ; \<Xi>, K, \<Gamma>1 \<turnstile> x :m t \<stileturn> \<Gamma>1'
+                       ; \<Xi>, K, \<Gamma>2 \<turnstile> y :m u \<stileturn> \<Gamma>2'
+                       \<rbrakk> \<Longrightarrow> \<Xi>, K, \<Gamma> \<turnstile> Tuple x y :m TProduct t u \<stileturn> merge_ctx K \<Gamma>1' \<Gamma>2'"
 
 | typing_min_split  : "\<lbrakk> K \<turnstile> \<Gamma> \<leadsto> \<Gamma>1 | \<Gamma>2
-                   ; \<Xi>, K, \<Gamma>1 \<turnstile> x :m TProduct t u \<stileturn> \<Gamma>1'
-                   ; \<Xi>, K, (Some t)#(Some u)#\<Gamma>2 \<turnstile> y :m t' \<stileturn> T' # U' # \<Gamma>2'
-                   \<rbrakk> \<Longrightarrow> \<Xi>, K, \<Gamma> \<turnstile> Split x y :m t' \<stileturn> merge_ctx K \<Gamma>1' \<Gamma>2'"
+                       ; \<Xi>, K, \<Gamma>1 \<turnstile> x :m TProduct t u \<stileturn> \<Gamma>1'
+                       ; \<Xi>, K, (Some t)#(Some u)#\<Gamma>2 \<turnstile> y :m t' \<stileturn> T' # U' # \<Gamma>2'
+                       \<rbrakk> \<Longrightarrow> \<Xi>, K, \<Gamma> \<turnstile> Split x y :m t' \<stileturn> merge_ctx K \<Gamma>1' \<Gamma>2'"
 
 | typing_min_let    : "\<lbrakk> K \<turnstile> \<Gamma> \<leadsto> \<Gamma>1 | \<Gamma>2
-                   ; \<Xi>, K, \<Gamma>1 \<turnstile> x :m t \<stileturn> \<Gamma>1'
-                   ; \<Xi>, K, (Some t # \<Gamma>2) \<turnstile> y :m u \<stileturn> T' # \<Gamma>2'
-                   \<rbrakk> \<Longrightarrow> \<Xi>, K, \<Gamma> \<turnstile> Let x y :m u \<stileturn> merge_ctx K \<Gamma>1' \<Gamma>2'"
+                       ; \<Xi>, K, \<Gamma>1 \<turnstile> x :m t \<stileturn> \<Gamma>1'
+                       ; \<Xi>, K, (Some t # \<Gamma>2) \<turnstile> y :m u \<stileturn> T' # \<Gamma>2'
+                       \<rbrakk> \<Longrightarrow> \<Xi>, K, \<Gamma> \<turnstile> Let x y :m u \<stileturn> merge_ctx K \<Gamma>1' \<Gamma>2'"
 
 | typing_min_letb   : "\<lbrakk> split_bang K is \<Gamma> \<Gamma>1 \<Gamma>2
-                   ; \<Xi>, K, \<Gamma>1 \<turnstile> x :m t \<stileturn> \<Gamma>1'
-                   ; \<Xi>, K, (Some t # \<Gamma>2) \<turnstile> y :m u \<stileturn> T' # \<Gamma>2'
-                   ; K \<turnstile> t :\<kappa> k
-                   ; E \<in> k
-                   \<rbrakk> \<Longrightarrow> \<Xi>, K, \<Gamma> \<turnstile> LetBang is x y :m u \<stileturn> merge_ctx_bang is K \<Gamma>1' \<Gamma>2'"
+                       ; \<Xi>, K, \<Gamma>1 \<turnstile> x :m t \<stileturn> \<Gamma>1'
+                       ; \<Xi>, K, (Some t # \<Gamma>2) \<turnstile> y :m u \<stileturn> T' # \<Gamma>2'
+                       ; K \<turnstile> t :\<kappa> k
+                       ; E \<in> k
+                       \<rbrakk> \<Longrightarrow> \<Xi>, K, \<Gamma> \<turnstile> LetBang is x y :m u \<stileturn> merge_ctx_bang K is \<Gamma>1' \<Gamma>2'"
 
 | typing_min_case   : "\<lbrakk> K \<turnstile> \<Gamma> \<leadsto> \<Gamma>1 | \<Gamma>2
-                   ; \<Xi>, K, \<Gamma>1 \<turnstile> x :m TSum ts \<stileturn> \<Gamma>1'
-                   ; (tag, (t,False)) \<in> set ts
-                   ; \<Xi>, K, (Some t # \<Gamma>2) \<turnstile> a :m u \<stileturn> T' # \<Gamma>2'
-                   ; \<Xi>, K, (Some (TSum (tagged_list_update tag (t, True) ts)) # \<Gamma>2) \<turnstile> b :m u \<stileturn> X' # \<Gamma>2'
-                   \<rbrakk> \<Longrightarrow> \<Xi>, K, \<Gamma> \<turnstile> Case x tag a b :m u \<stileturn> merge_ctx K \<Gamma>1' \<Gamma>2'"
+                       ; \<Xi>, K, \<Gamma>1 \<turnstile> x :m TSum ts \<stileturn> \<Gamma>1'
+                       ; (tag, (t,False)) \<in> set ts
+                       ; \<Xi>, K, (Some t # \<Gamma>2) \<turnstile> a :m u \<stileturn> T' # \<Gamma>2'
+                       ; \<Xi>, K, (Some (TSum (tagged_list_update tag (t, True) ts)) # \<Gamma>2) \<turnstile> b :m u \<stileturn> X' # \<Gamma>2'
+                       \<rbrakk> \<Longrightarrow> \<Xi>, K, \<Gamma> \<turnstile> Case x tag a b :m u \<stileturn> merge_ctx K \<Gamma>1' \<Gamma>2'"
 
 | typing_min_esac   : "\<lbrakk> \<Xi>, K, \<Gamma> \<turnstile> x :m TSum ts \<stileturn> \<Gamma>'
-                   ; [(_, (t,False))] = filter (HOL.Not \<circ> snd \<circ> snd) ts
-                   \<rbrakk> \<Longrightarrow> \<Xi>, K, \<Gamma> \<turnstile> Esac x :m t \<stileturn> \<Gamma>'"
+                       ; [(_, (t,False))] = filter (HOL.Not \<circ> snd \<circ> snd) ts
+                       \<rbrakk> \<Longrightarrow> \<Xi>, K, \<Gamma> \<turnstile> Esac x :m t \<stileturn> \<Gamma>'"
 
 | typing_min_if     : "\<lbrakk> K \<turnstile> \<Gamma> \<leadsto> \<Gamma>1 | \<Gamma>2
-                   ; \<Xi>, K, \<Gamma>1 \<turnstile> x :m TPrim Bool \<stileturn> \<Gamma>1'
-                   ; \<Xi>, K, \<Gamma>2 \<turnstile> a :m t \<stileturn> \<Gamma>2'
-                   ; \<Xi>, K, \<Gamma>2 \<turnstile> b :m t \<stileturn> \<Gamma>2'
-                   \<rbrakk> \<Longrightarrow> \<Xi>, K, \<Gamma> \<turnstile> If x a b :m t \<stileturn> merge_ctx K \<Gamma>1' \<Gamma>2'"
+                       ; \<Xi>, K, \<Gamma>1 \<turnstile> x :m TPrim Bool \<stileturn> \<Gamma>1'
+                       ; \<Xi>, K, \<Gamma>2 \<turnstile> a :m t \<stileturn> \<Gamma>2'
+                       ; \<Xi>, K, \<Gamma>2 \<turnstile> b :m t \<stileturn> \<Gamma>2'
+                       \<rbrakk> \<Longrightarrow> \<Xi>, K, \<Gamma> \<turnstile> If x a b :m t \<stileturn> merge_ctx K \<Gamma>1' \<Gamma>2'"
 
 | typing_min_prim   : "\<lbrakk> \<Xi>, K, \<Gamma> \<turnstile>* args :m map TPrim ts \<stileturn> \<Gamma>'
-                   ; prim_op_type oper = (ts,t)
-                   \<rbrakk> \<Longrightarrow> \<Xi>, K, \<Gamma> \<turnstile> Prim oper args :m TPrim t \<stileturn> \<Gamma>'"
+                       ; prim_op_type oper = (ts,t)
+                       \<rbrakk> \<Longrightarrow> \<Xi>, K, \<Gamma> \<turnstile> Prim oper args :m TPrim t \<stileturn> \<Gamma>'"
 
 | typing_min_lit    : "\<lbrakk> K \<turnstile> \<Gamma> consumed
-                   \<rbrakk> \<Longrightarrow> \<Xi>, K, \<Gamma> \<turnstile> Lit l :m TPrim (lit_type l) \<stileturn> empty (length \<Gamma>)"
+                       \<rbrakk> \<Longrightarrow> \<Xi>, K, \<Gamma> \<turnstile> Lit l :m TPrim (lit_type l) \<stileturn> empty (length \<Gamma>)"
 
 | typing_min_unit   : "\<lbrakk> K \<turnstile> \<Gamma> consumed
-                   \<rbrakk> \<Longrightarrow> \<Xi>, K, \<Gamma> \<turnstile> Unit :m TUnit \<stileturn> empty (length \<Gamma>)"
+                       \<rbrakk> \<Longrightarrow> \<Xi>, K, \<Gamma> \<turnstile> Unit :m TUnit \<stileturn> empty (length \<Gamma>)"
 
 | typing_min_struct : "\<lbrakk> \<Xi>, K, \<Gamma> \<turnstile>* es :m ts \<stileturn> \<Gamma>'
-                   \<rbrakk> \<Longrightarrow> \<Xi>, K, \<Gamma> \<turnstile> Struct ts es :m TRecord (zip ts (replicate (length ts) False)) Unboxed \<stileturn> \<Gamma>'"
+                       \<rbrakk> \<Longrightarrow> \<Xi>, K, \<Gamma> \<turnstile> Struct ts es :m TRecord (zip ts (replicate (length ts) False)) Unboxed \<stileturn> \<Gamma>'"
 
 | typing_min_member : "\<lbrakk> \<Xi>, K, \<Gamma> \<turnstile> e :m TRecord ts s \<stileturn> \<Gamma>'
-                   ; K \<turnstile> TRecord ts s :\<kappa> k
-                   ; S \<in> k
-                   ; f < length ts
-                   ; ts ! f = (t, False)
-                   \<rbrakk> \<Longrightarrow> \<Xi>, K, \<Gamma> \<turnstile> Member e f :m t \<stileturn> \<Gamma>'"
+                       ; K \<turnstile> TRecord ts s :\<kappa> k
+                       ; S \<in> k
+                       ; f < length ts
+                       ; ts ! f = (t, False)
+                       \<rbrakk> \<Longrightarrow> \<Xi>, K, \<Gamma> \<turnstile> Member e f :m t \<stileturn> \<Gamma>'"
 
 | typing_min_take   : "\<lbrakk> K \<turnstile> \<Gamma> \<leadsto> \<Gamma>1 | \<Gamma>2
-                   ; \<Xi>, K, \<Gamma>1 \<turnstile> e :m TRecord ts s \<stileturn> \<Gamma>1'
-                   ; sigil_perm s \<noteq> Some ReadOnly
-                   ; f < length ts
-                   ; ts ! f = (t, False)
-                   ; K \<turnstile> t :\<kappa> k
-                   ; S \<in> k \<or> taken
-                   ; \<Xi>, K, (Some t # Some (TRecord (ts [f := (t,taken)]) s) # \<Gamma>2) \<turnstile> e' :m u \<stileturn> T' # X' # \<Gamma>2'
-                   \<rbrakk> \<Longrightarrow> \<Xi>, K, \<Gamma> \<turnstile> Take e f e' :m u \<stileturn> merge_ctx K \<Gamma>1' \<Gamma>2'"
+                       ; \<Xi>, K, \<Gamma>1 \<turnstile> e :m TRecord ts s \<stileturn> \<Gamma>1'
+                       ; sigil_perm s \<noteq> Some ReadOnly
+                       ; f < length ts
+                       ; ts ! f = (t, False)
+                       ; K \<turnstile> t :\<kappa> k
+                       ; S \<in> k \<or> taken
+                       ; \<Xi>, K, (Some t # Some (TRecord (ts [f := (t,taken)]) s) # \<Gamma>2) \<turnstile> e' :m u \<stileturn> T' # X' # \<Gamma>2'
+                       \<rbrakk> \<Longrightarrow> \<Xi>, K, \<Gamma> \<turnstile> Take e f e' :m u \<stileturn> merge_ctx K \<Gamma>1' \<Gamma>2'"
 
 | typing_min_put    : "\<lbrakk> K \<turnstile> \<Gamma> \<leadsto> \<Gamma>1 | \<Gamma>2
-                   ; \<Xi>, K, \<Gamma>1 \<turnstile> e :m TRecord ts s \<stileturn> \<Gamma>1'
-                   ; sigil_perm s \<noteq> Some ReadOnly
-                   ; f < length ts
-                   ; ts ! f = (t, taken)
-                   ; K \<turnstile> t :\<kappa> k
-                   ; D \<in> k \<or> taken
-                   ; \<Xi>, K, \<Gamma>2 \<turnstile> e' :m t \<stileturn> \<Gamma>2'
-                   \<rbrakk> \<Longrightarrow> \<Xi>, K, \<Gamma> \<turnstile> Put e f e' :m TRecord (ts [f := (t,False)]) s \<stileturn> merge_ctx K \<Gamma>1' \<Gamma>2'"
+                       ; \<Xi>, K, \<Gamma>1 \<turnstile> e :m TRecord ts s \<stileturn> \<Gamma>1'
+                       ; sigil_perm s \<noteq> Some ReadOnly
+                       ; f < length ts
+                       ; ts ! f = (t, taken)
+                       ; K \<turnstile> t :\<kappa> k
+                       ; D \<in> k \<or> taken
+                       ; \<Xi>, K, \<Gamma>2 \<turnstile> e' :m t \<stileturn> \<Gamma>2'
+                       \<rbrakk> \<Longrightarrow> \<Xi>, K, \<Gamma> \<turnstile> Put e f e' :m TRecord (ts [f := (t,False)]) s \<stileturn> merge_ctx K \<Gamma>1' \<Gamma>2'"
 
 | typing_min_all_empty : "\<Xi>, K, empty n \<turnstile>* [] :m [] \<stileturn> empty n"
 
 | typing_min_all_cons  : "\<lbrakk> K \<turnstile> \<Gamma> \<leadsto> \<Gamma>1 | \<Gamma>2
-                      ; \<Xi>, K, \<Gamma>1 \<turnstile>  e  :m t \<stileturn> \<Gamma>1'
-                      ; \<Xi>, K, \<Gamma>2 \<turnstile>* es :m ts \<stileturn>  \<Gamma>2'
-                      \<rbrakk> \<Longrightarrow> \<Xi>, K, \<Gamma> \<turnstile>* (e # es) :m (t # ts) \<stileturn> merge_ctx K \<Gamma>1' \<Gamma>2'"
+                          ; \<Xi>, K, \<Gamma>1 \<turnstile>  e  :m t \<stileturn> \<Gamma>1'
+                          ; \<Xi>, K, \<Gamma>2 \<turnstile>* es :m ts \<stileturn>  \<Gamma>2'
+                          \<rbrakk> \<Longrightarrow> \<Xi>, K, \<Gamma> \<turnstile>* (e # es) :m (t # ts) \<stileturn> merge_ctx K \<Gamma>1' \<Gamma>2'"
+
+
+lemma typing_min_to_kinding:
+  shows "\<Xi>, K, \<Gamma> \<turnstile>  e  :m t  \<stileturn> \<Gamma>' \<Longrightarrow> K \<turnstile>  t  wellformed"
+    and "\<Xi>, K, \<Gamma> \<turnstile>* es :m ts \<stileturn> \<Gamma>' \<Longrightarrow> K \<turnstile>* ts wellformed"
+proof (induct rule: typing_minimal_typing_minimal_all.inducts)
+  case typing_min_var then show ?case
+    by (fastforce
+        dest: weakening_preservation_some weakening_nth
+        simp: empty_length
+        elim: weakening_comp.cases)
+next case typing_min_fun    then show ?case
+    by (fastforce intro: kinding_kinding_all_kinding_record.intros substitutivity)
+next case typing_min_afun   then show ?case
+    by (fastforce intro: kinding_kinding_all_kinding_record.intros substitutivity)
+next case typing_min_con    then show ?case
+    by (fastforce
+        simp add: kinding_all_set
+        intro!: kinding_kinding_all_kinding_record.intros)
+next case typing_min_esac   then show ?case
+    by (fastforce
+        dest: filtered_member
+        elim: kinding.cases
+        simp add: kinding_all_set)
+next case typing_min_member then show ?case
+    by (fastforce intro: kinding_record_wellformed_nth)
+next case typing_min_struct then show ?case 
+    by (clarsimp , intro exI kind_trec kinding_all_record , simp_all add: kind_top)
+next case typing_min_put    then show ?case
+    by (fastforce intro: kinding_kinding_all_kinding_record.intros  kinding_record_update)
+qed (auto intro: supersumption kinding_kinding_all_kinding_record.intros)
+
+
+lemma
+  shows "\<Xi>, K, \<Gamma> \<turnstile> e :m t \<stileturn> \<Gamma>' \<Longrightarrow> K \<turnstile> \<Gamma> \<leadsto>w \<Gamma>'"
+    and "\<Xi>, K, \<Gamma> \<turnstile>* es :m ts \<stileturn> \<Gamma>' \<Longrightarrow> K \<turnstile> \<Gamma> \<leadsto>w \<Gamma>'"
+proof (induct rule: typing_minimal_typing_minimal_all.inducts)
+  case (typing_min_app K \<Gamma> \<Gamma>1 \<Gamma>2 \<Xi> a x y \<Gamma>1' b \<Gamma>2')
+
+  obtain \<Gamma>' where weaken_and_split\<Gamma>:
+    "K \<turnstile> \<Gamma> \<leadsto>w \<Gamma>' \<and> K \<turnstile> \<Gamma>' \<leadsto> \<Gamma>1' | \<Gamma>2'"
+    using weaken_and_split typing_min_app.hyps 
+    by blast
+  then have \<Gamma>_is: "\<Gamma> = merge_ctx K \<Gamma>1 \<Gamma>2"
+    by (simp add: merge_ctx_correct_on_splits typing_min_app.hyps)
+
+  have subrules_wellformed:
+    "\<And>y. Some y \<in> set \<Gamma>1 \<Longrightarrow> K \<turnstile> y wellformed"
+    "\<And>y. Some y \<in> set \<Gamma>2 \<Longrightarrow> K \<turnstile> y wellformed"
+    using typing_min_app.hyps weakening_implies_wellformed by force+
+
+  show ?case
+    using \<Gamma>_is weaken_and_split\<Gamma> weakening_refl subrules_wellformed weakening_implies_wellformed
+    by auto
+next
+  case (typing_min_tuple K \<Gamma> \<Gamma>1 \<Gamma>2 \<Xi> x t \<Gamma>1' y u \<Gamma>2')
+
+  obtain \<Gamma>' where weaken_and_split\<Gamma>:
+    "K \<turnstile> \<Gamma> \<leadsto>w \<Gamma>' \<and> K \<turnstile> \<Gamma>' \<leadsto> \<Gamma>1' | \<Gamma>2'"
+    using weaken_and_split typing_min_tuple.hyps 
+    by blast
+  moreover then have \<Gamma>_\<Gamma>'_simps: "\<Gamma> = merge_ctx K \<Gamma>1 \<Gamma>2"
+          "\<Gamma>' = merge_ctx K \<Gamma>1' \<Gamma>2'"
+    by (simp add: merge_ctx_correct_on_splits typing_min_tuple.hyps)+
+  ultimately show ?case
+    by auto
+next
+  case (typing_min_split K \<Gamma> \<Gamma>1 \<Gamma>2 \<Xi> x t u \<Gamma>1' y t' T' U' \<Gamma>2')
+
+  have "K \<turnstile> \<Gamma>2 \<leadsto>w \<Gamma>2'"
+    using typing_min_split
+    by (simp add: weakening_def)
+  then obtain \<Gamma>' where weaken_and_split\<Gamma>:
+    "K \<turnstile> \<Gamma> \<leadsto>w \<Gamma>'"
+    "K \<turnstile> \<Gamma>' \<leadsto> \<Gamma>1' | \<Gamma>2'"
+    using weaken_and_split typing_min_split
+    by meson
+  then have \<Gamma>'_is: "\<Gamma>' = merge_ctx K \<Gamma>1' \<Gamma>2'"
+    by (simp add: merge_ctx_correct_on_splits weaken_and_split\<Gamma>(2))
+
+  show ?case
+    using \<Gamma>'_is weaken_and_split\<Gamma> by fast
+next
+  case (typing_min_let K \<Gamma> \<Gamma>1 \<Gamma>2 \<Xi> x t \<Gamma>1' y u T' \<Gamma>2')
+
+  have weaken_\<Gamma>2:
+    "K \<turnstile> \<Gamma>2 \<leadsto>w \<Gamma>2'"
+    using typing_min_let
+    by (simp add: weakening_def)
+  then obtain \<Gamma>' where weaken_and_split\<Gamma>:
+    "K \<turnstile> \<Gamma> \<leadsto>w \<Gamma>'"
+    "K \<turnstile> \<Gamma>' \<leadsto> \<Gamma>1' | \<Gamma>2'"
+    using weaken_and_split typing_min_let
+    by meson
+  then have \<Gamma>'_is: "\<Gamma>' = merge_ctx K \<Gamma>1' \<Gamma>2'"
+    by (simp add: merge_ctx_correct_on_splits weaken_and_split\<Gamma>(2))
+
+  then show ?case
+    using \<Gamma>'_is weaken_and_split\<Gamma> by fast
+next
+  case (typing_min_letb K "is" \<Gamma> \<Gamma>1 \<Gamma>2 \<Xi> x t \<Gamma>1' y u T' \<Gamma>2' k)
+
+  have weaken_\<Gamma>2:
+    "K \<turnstile> \<Gamma>2 \<leadsto>w \<Gamma>2'"
+    using typing_min_letb
+    by (simp add: weakening_def)
+  then obtain \<Gamma>' where weaken_and_split\<Gamma>:
+    "K \<turnstile> \<Gamma> \<leadsto>w \<Gamma>'"
+    "K \<turnstile> \<Gamma>' \<leadsto> \<Gamma>1' | \<Gamma>2'"
+    using weaken_and_split typing_min_letb
+    sorry
+  then have \<Gamma>'_is: "\<Gamma>' = merge_ctx K \<Gamma>1' \<Gamma>2'"
+    by (simp add: merge_ctx_correct_on_splits weaken_and_split\<Gamma>(2))
+
+  then show ?case
+    using \<Gamma>'_is weaken_and_split\<Gamma> sorry
+
+next
+  case (typing_min_case K \<Gamma> \<Gamma>1 \<Gamma>2 \<Xi> x ts \<Gamma>1' tag t a u T' \<Gamma>2' b X')
+  then show ?case sorry
+next
+case (typing_min_if K \<Gamma> \<Gamma>1 \<Gamma>2 \<Xi> x \<Gamma>1' a t \<Gamma>2' b)
+  then show ?case sorry
+next
+  case (typing_min_take K \<Gamma> \<Gamma>1 \<Gamma>2 \<Xi> e ts s \<Gamma>1' f t k taken e' u T' X' \<Gamma>2')
+  then show ?case sorry
+next
+  case (typing_min_put K \<Gamma> \<Gamma>1 \<Gamma>2 \<Xi> e ts s \<Gamma>1' f t taken k e' \<Gamma>2')
+then show ?case sorry
+next
+  case (typing_min_all_empty \<Xi> K n)
+  then show ?case sorry
+next
+  case (typing_min_all_cons K \<Gamma> \<Gamma>1 \<Gamma>2 \<Xi> e t \<Gamma>1' es ts \<Gamma>2')
+  then show ?case sorry
+qed simp+
 
 lemma minimal_typing_soundness:
+(*
+when we remove the \<Gamma>, we will need the full lemma, for now, we get it for free
   shows "\<Xi>, K, \<Gamma> \<turnstile> e : t \<Longrightarrow> \<exists>\<Gamma>'. (\<Xi>, K, \<Gamma> \<turnstile> e :m t \<stileturn> \<Gamma>') \<and> (K \<turnstile> \<Gamma> \<leadsto>w  \<Gamma>')"
     and "\<Xi>, K, \<Gamma> \<turnstile>* es : ts \<Longrightarrow> \<exists>\<Gamma>'. (\<Xi>, K, \<Gamma> \<turnstile>* es :m ts \<stileturn> \<Gamma>') \<and> (K \<turnstile> \<Gamma> \<leadsto>w  \<Gamma>')"
+*)
+  shows "\<Xi>, K, \<Gamma> \<turnstile> e : t \<Longrightarrow> \<exists>\<Gamma>'. (\<Xi>, K, \<Gamma> \<turnstile> e :m t \<stileturn> \<Gamma>')"
+    and "\<Xi>, K, \<Gamma> \<turnstile>* es : ts \<Longrightarrow> \<exists>\<Gamma>'. (\<Xi>, K, \<Gamma> \<turnstile>* es :m ts \<stileturn> \<Gamma>')"
 proof (induct rule: typing_typing_all.inducts)
-  case (typing_var K \<Gamma> i t \<Xi>)
+case (typing_var K \<Gamma> i t \<Xi>)
   then show ?case sorry
+next
+  case (typing_afun \<Xi> f K' t u K ts \<Gamma>)
+  then show ?case sorry
+next
+  case (typing_fun \<Xi> K' t f u K \<Gamma> ts)
+  then show ?case sorry
+next
+  case (typing_app K \<Gamma> \<Gamma>1 \<Gamma>2 \<Xi> a x y b)
+  then show ?case sorry
+next
+  case (typing_con \<Xi> K \<Gamma> x t tag ts ts')
+  then show ?case sorry
+next
+  case (typing_cast \<Xi> K \<Gamma> e \<tau> \<tau>')
+  then show ?case sorry
+next
+  case (typing_tuple K \<Gamma> \<Gamma>1 \<Gamma>2 \<Xi> t T u U)
+  then show ?case sorry
+next
+  case (typing_split K \<Gamma> \<Gamma>1 \<Gamma>2 \<Xi> x t u y t')
+  then show ?case sorry
+next
+  case (typing_let K \<Gamma> \<Gamma>1 \<Gamma>2 \<Xi> x t y u)
+  then show ?case sorry
+next
+  case (typing_letb K "is" \<Gamma> \<Gamma>1 \<Gamma>2 \<Xi> x t y u k)
+  then show ?case sorry
+next
+  case (typing_case K \<Gamma> \<Gamma>1 \<Gamma>2 \<Xi> x ts tag t a u b)
+  then show ?case sorry
+next
+  case (typing_esac \<Xi> K \<Gamma> x ts uu t)
+  then show ?case sorry
+next
+  case (typing_if K \<Gamma> \<Gamma>1 \<Gamma>2 \<Xi> x a t b)
+  then show ?case sorry
+next
+  case (typing_prim \<Xi> K \<Gamma> args ts oper t)
+  then show ?case sorry
+next
+  case (typing_lit K \<Gamma> \<Xi> l)
+  then show ?case sorry
+next
+  case (typing_unit K \<Gamma> \<Xi>)
+  then show ?case sorry
+next
+  case (typing_struct \<Xi> K \<Gamma> es ts)
+  then show ?case sorry
+next
+  case (typing_member \<Xi> K \<Gamma> e ts s k f t)
+  then show ?case sorry
+next
+  case (typing_take K \<Gamma> \<Gamma>1 \<Gamma>2 \<Xi> e ts s f t k taken e' u)
+  then show ?case sorry
+next
+  case (typing_put K \<Gamma> \<Gamma>1 \<Gamma>2 \<Xi> e ts s f t taken k e')
+  then show ?case sorry
+next
+  case (typing_all_empty \<Xi> K n)
+  then show ?case sorry
+next
+  case (typing_all_cons K \<Gamma> \<Gamma>1 \<Gamma>2 \<Xi> e t es ts)
+  then show ?case sorry
+qed
+
+(*  case (typing_var K \<Gamma> i t \<Xi>)
+  then show ?case
+    using typing_min_var by blast
 next
   case (typing_afun \<Xi> f K' t u K ts \<Gamma>)
   then have "\<Xi>, K, \<Gamma> \<turnstile> AFun f ts :m instantiate ts (TFun t u) \<stileturn> Cogent.empty (length \<Gamma>)"
@@ -260,10 +500,12 @@ next
   case (typing_all_cons K \<Gamma> \<Gamma>1 \<Gamma>2 \<Xi> e t es ts)
   then show ?case sorry
 qed
+*)
 
 lemma minimal_typing_completeness:
   assumes "\<Xi>, K, \<Gamma> \<turnstile> e :m t \<stileturn> \<Gamma>'"
-  shows "\<Xi>, K, \<Gamma>' \<turnstile> e : t"
+  shows "\<Xi>, K, \<Gamma> \<turnstile> e : t"
+    and "\<Xi>, K, \<Gamma>' \<turnstile> e : t"
   sorry
 
 lemma minimal_typing_generates_minimal_weakened:
